@prefix : <https://github.com/w3c/wot-discovery#> .
@prefix owl: <http://www.w3.org/2002/07/owl#> .
@prefix rdf: <http://www.w3.org/1999/02/22-rdf-syntax-ns#> .
@prefix rdfs: <http://www.w3.org/2000/01/rdf-schema#> .
@prefix xml: <http://www.w3.org/XML/1998/namespace> .
@prefix xsd: <http://www.w3.org/2001/XMLSchema#> .
@prefix dc: <http://purl.org/dc/elements/1.1/> .
@prefix dcterms: <http://purl.org/dc/terms/> .
@prefix vann: <http://purl.org/vocab/vann/> .
@prefix td: <https://www.w3.org/2019/wot/td#> .
@prefix did: <https://www.w3.org/ns/did#> .
@prefix schema: <http://schema.org/> .

: rdf:type owl:Ontology ;
	dc:creator "Andrea Cimmino" ;
	dc:creator "Farshid Tavakolizadeh" ;
	owl:versionInfo "0.2.0-a1" ;
	# TODO: Add proper owl:priorVersion
	owl:priorVersion "https://raw.githubusercontent.com/w3c/wot-discovery/main/publication/6-resources/ontology/discovery-ontology.ttl";
	vann:changes "Script used to render HTML from TTL. TTL updated to include annotations and comments, and defining default namespace." ;
	vann:preferredNamespacePrefix "discovery" ;
	vann:preferredNamespaceUri "https://github.com/w3c/wot-discovery#" ;
	dc:title "WoT discovery ontology" ;
	dc:description "Ontology code created by Chowlk" .

#################################################################
# Object Properties
#################################################################

### discovery:hasRegistrationInformation
:hasRegistrationInformation rdf:type owl:ObjectProperty ;
	rdfs:comment "Used to provide information on the registration with a Thing Description Directory in a TD."@en ;
	rdfs:domain td:Thing ;
	rdfs:range :RegistrationInformation ;
	rdfs:label "registration" .

### discovery:nextThingCollection
:nextThingCollection rdf:type owl:ObjectProperty;
	rdfs:comment "Used to provide a link for retrieving a URL for retrieving the next page of a ThingCollection. "@en ;
	rdfs:domain :ThingCollection;
	rdfs:range :ThingCollection;
	rdfs:label "next ThingCollection" .


### discovery:hasCollectionMember
:hasCollectionMember rdf:type owl:ObjectProperty;
	rdfs:comment "The array of Thing Descriptions contained in a ThingCollection."@en ;
	rdfs:domain :ThingCollection;
	rdfs:range td:Thing;
	rdfs:label "ThingCollection members" .

#################################################################

# Data Properties

#################################################################

### discovery:dateCreated
:dateCreated rdf:type owl:DatatypeProperty ;
	rdfs:comment "Provides the absolute time when the TD instance was created inside the directory. "@en ;
	rdfs:domain :RegistrationInformation ;
	rdfs:range xsd:dateTime ;
	rdfs:label "created"@en .

### discovery:dateModified
:dateModified rdf:type owl:DatatypeProperty ;
	rdfs:comment "Provides the absolute time when the TD instance was last modified inside the directory."@en ;
	rdfs:domain :RegistrationInformation ;
	rdfs:range xsd:dateTime ;
	rdfs:label "modified"@en .

### discovery:expires
:expires rdf:type owl:DatatypeProperty ;
	rdfs:comment "Provides the absolute time when the TD instance registration expires."@en ;
	rdfs:domain :RegistrationInformation ;
	rdfs:range xsd:dateTime ;
	rdfs:label "expires"@en .

### discovery:ttl
:ttl rdf:type owl:DatatypeProperty ;
	rdfs:comment "Time-to-live: relative amount of time in seconds from the registration time until when the TD instance registration expires."@en ;
	rdfs:domain :RegistrationInformation ;
	rdfs:range xsd:unsignedInt ;
	rdfs:label "ttl"@en .

### discovery:retrieve
:retrieved rdf:type owl:DatatypeProperty ;
	rdfs:comment "The absolute time at which the TD was retrieved from the server."@en ;
	rdfs:domain :RegistrationInformation ;
	rdfs:range xsd:dateTime ;
	rdfs:label "retrieved"@en .

### discovery:contains
:contains rdf:type owl:DatatypeProperty ;
	rdfs:comment "Refers to the total number of Things contained in a ThingCollection."@en ;
	rdfs:domain :ThingCollection;
	rdfs:range xsd:integer;
	rdfs:label "total number of things contained in the collection"@en .
#################################################################

# Classes

#################################################################

### discovery:RegistrationInformation
:RegistrationInformation rdf:type owl:Class ;
	rdfs:comment "Associated with TDs that are stored in a directory, providing additional information set during the registration with the TDD."@en ;
	rdfs:label "RegistrationInformation" .

### discovery:ThingLink
:ThingLink rdf:type owl:Class ;
	rdfs:comment "Class of Thing Descriptions that refer to another TD."@en ;
	rdfs:label "ThingLink" ;
	rdfs:subClassOf td:Thing .

### discovery:ThingDirectory
:ThingDirectory rdf:type owl:Class ;
	rdfs:comment "Class of Thing Descriptions that describe a Thing Description Directory."@en ;
	rdfs:label "ThingDirectory" ;
	rdfs:subClassOf td:Thing .

### discovery:ThingCollection
:ThingCollection rdf:type owl:Class ;
	rdfs:comment "A collection of TDs containing pagination information."@en ;
	rdfs:label "ThingCollection".

### discovery:WotThingDIDService
:WotThingDIDService rdf:type owl:Class ;
	rdfs:comment "Class used in DID documents that labels a URL for a service returning a WoT TD";
	rdfs:subClassOf did:Service ;
	rdfs:label "WotThingDIDService" .

### discovery:WotDirectoryDIDService
:WotDirectoryDIDService rdf:type owl:Class ;
	rdfs:comment "Class used in DID documents that labels a URL for a service returning a WoT TD that must describe a WoT TD Directory";
        rdfs:subClassOf did:Service ;
	rdfs:label "WotDirectoryDIDService" .


#################################################################
# Instances
#################################################################

#################################################################
# General Axioms
#################################################################
